section \<open>Using Hoare Logic\<close>

theory Hoare_Ex
  imports Hoare
begin

subsection \<open>State spaces\<close>

text \<open>
  First of all we provide a store of program variables that occur in any of
  the programs considered later. Slightly unexpected things may happen when
  attempting to work with undeclared variables.
\<close>

record vars =
  I :: nat
  M :: nat
  N :: nat
  S :: nat

text \<open>
  While all of our variables happen to have the same type, nothing would
  prevent us from working with many-sorted programs as well, or even
  polymorphic ones. Also note that Isabelle/HOL's extensible record types even
  provides simple means to extend the state space later.
\<close>


subsection \<open>Basic examples\<close>

text \<open>
  We look at few trivialities involving assignment and sequential composition,
  in order to get an idea of how to work with our formulation of Hoare Logic.

  \<^medskip>
  Using the basic \<open>assign\<close> rule directly is a bit cumbersome.
\<close>

lemma "\<turnstile> \<lbrace>\<acute>(N_update (\<lambda>_. (2 * \<acute>N))) \<in> \<lbrace>\<acute>N = 10\<rbrace>\<rbrace> \<acute>N := 2 * \<acute>N \<lbrace>\<acute>N = 10\<rbrace>"
  by (rule assign)

text \<open>
  Certainly we want the state modification already done, e.g.\ by
  simplification. The \<open>hoare\<close> method performs the basic state update for us;
  we may apply the Simplifier afterwards to achieve ``obvious'' consequences
  as well.
\<close>

lemma "\<turnstile> \<lbrace>True\<rbrace> \<acute>N := 10 \<lbrace>\<acute>N = 10\<rbrace>"
  by hoare

lemma "\<turnstile> \<lbrace>2 * \<acute>N = 10\<rbrace> \<acute>N := 2 * \<acute>N \<lbrace>\<acute>N = 10\<rbrace>"
  by hoare

lemma "\<turnstile> \<lbrace>\<acute>N = 5\<rbrace> \<acute>N := 2 * \<acute>N \<lbrace>\<acute>N = 10\<rbrace>"
  by hoare simp

lemma "\<turnstile> \<lbrace>\<acute>N + 1 = a + 1\<rbrace> \<acute>N := \<acute>N + 1 \<lbrace>\<acute>N = a + 1\<rbrace>"
  by hoare

lemma "\<turnstile> \<lbrace>\<acute>N = a\<rbrace> \<acute>N := \<acute>N + 1 \<lbrace>\<acute>N = a + 1\<rbrace>"
  by hoare simp

lemma "\<turnstile> \<lbrace>a = a \<and> b = b\<rbrace> \<acute>M := a; \<acute>N := b \<lbrace>\<acute>M = a \<and> \<acute>N = b\<rbrace>"
  by hoare

lemma "\<turnstile> \<lbrace>True\<rbrace> \<acute>M := a; \<acute>N := b \<lbrace>\<acute>M = a \<and> \<acute>N = b\<rbrace>"
  by hoare

lemma
  "\<turnstile> \<lbrace>\<acute>M = a \<and> \<acute>N = b\<rbrace>
      \<acute>I := \<acute>M; \<acute>M := \<acute>N; \<acute>N := \<acute>I
      \<lbrace>\<acute>M = b \<and> \<acute>N = a\<rbrace>"
  by hoare simp

text \<open>
  It is important to note that statements like the following one can only be
  proven for each individual program variable. Due to the extra-logical nature
  of record fields, we cannot formulate a theorem relating record selectors
  and updates schematically.
\<close>

lemma "\<turnstile> \<lbrace>\<acute>N = a\<rbrace> \<acute>N := \<acute>N \<lbrace>\<acute>N = a\<rbrace>"
  by hoare

lemma "\<turnstile> \<lbrace>\<acute>x = a\<rbrace> \<acute>x := \<acute>x \<lbrace>\<acute>x = a\<rbrace>"
  oops

lemma
  "Valid {s. x s = a} (Basic (\<lambda>s. x_update (x s) s)) {s. x s = n}"
  \<comment> \<open>same statement without concrete syntax\<close>
  oops


text \<open>
  In the following assignments we make use of the consequence rule in order to
  achieve the intended precondition. Certainly, the \<open>hoare\<close> method is able to
  handle this case, too.
\<close>

lemma "\<turnstile> \<lbrace>\<acute>M = \<acute>N\<rbrace> \<acute>M := \<acute>M + 1 \<lbrace>\<acute>M \<noteq> \<acute>N\<rbrace>"
proof -
  have "\<lbrace>\<acute>M = \<acute>N\<rbrace> \<subseteq> \<lbrace>\<acute>M + 1 \<noteq> \<acute>N\<rbrace>"
    by auto
  also have "\<turnstile> \<dots> \<acute>M := \<acute>M + 1 \<lbrace>\<acute>M \<noteq> \<acute>N\<rbrace>"
    by hoare
  finally show ?thesis .
qed

lemma "\<turnstile> \<lbrace>\<acute>M = \<acute>N\<rbrace> \<acute>M := \<acute>M + 1 \<lbrace>\<acute>M \<noteq> \<acute>N\<rbrace>"
proof -
  have "m = n \<longrightarrow> m + 1 \<noteq> n" for m n :: nat
      \<comment> \<open>inclusion of assertions expressed in ``pure'' logic,\<close>
      \<comment> \<open>without mentioning the state space\<close>
    by simp
  also have "\<turnstile> \<lbrace>\<acute>M + 1 \<noteq> \<acute>N\<rbrace> \<acute>M := \<acute>M + 1 \<lbrace>\<acute>M \<noteq> \<acute>N\<rbrace>"
    by hoare
  finally show ?thesis .
qed

lemma "\<turnstile> \<lbrace>\<acute>M = \<acute>N\<rbrace> \<acute>M := \<acute>M + 1 \<lbrace>\<acute>M \<noteq> \<acute>N\<rbrace>"
  by hoare simp


subsection \<open>Multiplication by addition\<close>

text \<open>
  We now do some basic examples of actual \<^verbatim>\<open>WHILE\<close> programs. This one is a
  loop for calculating the product of two natural numbers, by iterated
  addition. We first give detailed structured proof based on single-step Hoare
  rules.
\<close>

lemma
  "\<turnstile> \<lbrace>\<acute>M = 0 \<and> \<acute>S = 0\<rbrace>
      WHILE \<acute>M \<noteq> a
      DO \<acute>S := \<acute>S + b; \<acute>M := \<acute>M + 1 OD
      \<lbrace>\<acute>S = a * b\<rbrace>"
proof -
  let "\<turnstile> _ ?while _" = ?thesis
  let "\<lbrace>\<acute>?inv\<rbrace>" = "\<lbrace>\<acute>S = \<acute>M * b\<rbrace>"

  have "\<lbrace>\<acute>M = 0 \<and> \<acute>S = 0\<rbrace> \<subseteq> \<lbrace>\<acute>?inv\<rbrace>" by auto
  also have "\<turnstile> \<dots> ?while \<lbrace>\<acute>?inv \<and> \<not> (\<acute>M \<noteq> a)\<rbrace>"
  proof
    let ?c = "\<acute>S := \<acute>S + b; \<acute>M := \<acute>M + 1"
    have "\<lbrace>\<acute>?inv \<and> \<acute>M \<noteq> a\<rbrace> \<subseteq> \<lbrace>\<acute>S + b = (\<acute>M + 1) * b\<rbrace>"
      by auto
    also have "\<turnstile> \<dots> ?c \<lbrace>\<acute>?inv\<rbrace>" by hoare
    finally show "\<turnstile> \<lbrace>\<acute>?inv \<and> \<acute>M \<noteq> a\<rbrace> ?c \<lbrace>\<acute>?inv\<rbrace>" .
  qed
  also have "\<dots> \<subseteq> \<lbrace>\<acute>S = a * b\<rbrace>" by auto
  finally show ?thesis .
qed

text \<open>
  The subsequent version of the proof applies the \<open>hoare\<close> method to reduce the
  Hoare statement to a purely logical problem that can be solved fully
  automatically. Note that we have to specify the \<^verbatim>\<open>WHILE\<close> loop invariant in
  the original statement.
\<close>

lemma
  "\<turnstile> \<lbrace>\<acute>M = 0 \<and> \<acute>S = 0\<rbrace>
      WHILE \<acute>M \<noteq> a
      INV \<lbrace>\<acute>S = \<acute>M * b\<rbrace>
      DO \<acute>S := \<acute>S + b; \<acute>M := \<acute>M + 1 OD
      \<lbrace>\<acute>S = a * b\<rbrace>"
  by hoare auto


subsection \<open>Summing natural numbers\<close>

text \<open>
  We verify an imperative program to sum natural numbers up to a given limit.
  First some functional definition for proper specification of the problem.

  \<^medskip>
  The following proof is quite explicit in the individual steps taken, with
  the \<open>hoare\<close> method only applied locally to take care of assignment and
  sequential composition. Note that we express intermediate proof obligation
  in pure logic, without referring to the state space.
\<close>

theorem
  "\<turnstile> \<lbrace>True\<rbrace>
      \<acute>S := 0; \<acute>I := 1;
      WHILE \<acute>I \<noteq> n
      DO
        \<acute>S := \<acute>S + \<acute>I;
        \<acute>I := \<acute>I + 1
      OD
      \<lbrace>\<acute>S = (\<Sum>j<n. j)\<rbrace>"
  (is "\<turnstile> _ (_; ?while) _")
proof -
  let ?sum = "\<lambda>k::nat. \<Sum>j<k. j"
  let ?inv = "\<lambda>s i::nat. s = ?sum i"

  have "\<turnstile> \<lbrace>True\<rbrace> \<acute>S := 0; \<acute>I := 1 \<lbrace>?inv \<acute>S \<acute>I\<rbrace>"
  proof -
    have "True \<longrightarrow> 0 = ?sum 1"
      by simp
    also have "\<turnstile> \<lbrace>\<dots>\<rbrace> \<acute>S := 0; \<acute>I := 1 \<lbrace>?inv \<acute>S \<acute>I\<rbrace>"
      by hoare
    finally show ?thesis .
  qed
  also have "\<turnstile> \<dots> ?while \<lbrace>?inv \<acute>S \<acute>I \<and> \<not> \<acute>I \<noteq> n\<rbrace>"
  proof
    let ?body = "\<acute>S := \<acute>S + \<acute>I; \<acute>I := \<acute>I + 1"
    have "?inv s i \<and> i \<noteq> n \<longrightarrow> ?inv (s + i) (i + 1)" for s i
      by simp
    also have "\<turnstile> \<lbrace>\<acute>S + \<acute>I = ?sum (\<acute>I + 1)\<rbrace> ?body \<lbrace>?inv \<acute>S \<acute>I\<rbrace>"
      by hoare
    finally show "\<turnstile> \<lbrace>?inv \<acute>S \<acute>I \<and> \<acute>I \<noteq> n\<rbrace> ?body \<lbrace>?inv \<acute>S \<acute>I\<rbrace>" .
  qed
  also have "s = ?sum i \<and> \<not> i \<noteq> n \<longrightarrow> s = ?sum n" for s i
    by simp
  finally show ?thesis .
qed

text \<open>
  The next version uses the \<open>hoare\<close> method, while still explaining the
  resulting proof obligations in an abstract, structured manner.
\<close>

theorem
  "\<turnstile> \<lbrace>True\<rbrace>
      \<acute>S := 0; \<acute>I := 1;
      WHILE \<acute>I \<noteq> n
      INV \<lbrace>\<acute>S = (\<Sum>j<\<acute>I. j)\<rbrace>
      DO
        \<acute>S := \<acute>S + \<acute>I;
        \<acute>I := \<acute>I + 1
      OD
      \<lbrace>\<acute>S = (\<Sum>j<n. j)\<rbrace>"
proof -
  let ?sum = "\<lambda>k::nat. \<Sum>j<k. j"
  let ?inv = "\<lambda>s i::nat. s = ?sum i"
  show ?thesis
  proof hoare
    show "?inv 0 1" by simp
    show "?inv (s + i) (i + 1)" if "?inv s i \<and> i \<noteq> n" for s i
      using that by simp
    show "s = ?sum n" if "?inv s i \<and> \<not> i \<noteq> n" for s i
      using that by simp
  qed
qed

text \<open>
  Certainly, this proof may be done fully automatic as well, provided that the
  invariant is given beforehand.
\<close>

theorem
  "\<turnstile> \<lbrace>True\<rbrace>
      \<acute>S := 0; \<acute>I := 1;
      WHILE \<acute>I \<noteq> n
      INV \<lbrace>\<acute>S = (\<Sum>j<\<acute>I. j)\<rbrace>
      DO
        \<acute>S := \<acute>S + \<acute>I;
        \<acute>I := \<acute>I + 1
      OD
      \<lbrace>\<acute>S = (\<Sum>j<n. j)\<rbrace>"
  by hoare auto


subsection \<open>Time\<close>

text \<open>
  A simple embedding of time in Hoare logic: function \<open>timeit\<close> inserts an
  extra variable to keep track of the elapsed time.
\<close>

record tstate = time :: nat

type_synonym 'a time = "\<lparr>time :: nat, \<dots> :: 'a\<rparr>"

primrec timeit :: "'a time com \<Rightarrow> 'a time com"
  where
    "timeit (Basic f) = (Basic f; Basic(\<lambda>s. s\<lparr>time := Suc (time s)\<rparr>))"
  | "timeit (c1; c2) = (timeit c1; timeit c2)"
  | "timeit (Cond b c1 c2) = Cond b (timeit c1) (timeit c2)"
  | "timeit (While b iv c) = While b iv (timeit c)"

record tvars = tstate +
  I :: nat
  J :: nat

lemma lem: "(0::nat) < n \<Longrightarrow> n + n \<le> Suc (n * n)"
  by (induct n) simp_all

lemma
  "\<turnstile> \<lbrace>i = \<acute>I \<and> \<acute>time = 0\<rbrace>
    (timeit
      (WHILE \<acute>I \<noteq> 0
        INV \<lbrace>2 *\<acute> time + \<acute>I * \<acute>I + 5 * \<acute>I = i * i + 5 * i\<rbrace>
        DO
          \<acute>J := \<acute>I;
          WHILE \<acute>J \<noteq> 0
          INV \<lbrace>0 < \<acute>I \<and> 2 * \<acute>time + \<acute>I * \<acute>I + 3 * \<acute>I + 2 * \<acute>J - 2 = i * i + 5 * i\<rbrace>
          DO \<acute>J := \<acute>J - 1 OD;
          \<acute>I := \<acute>I - 1
        OD))
    \<lbrace>2 * \<acute>time = i * i + 5 * i\<rbrace>"
  apply simp
  apply hoare
      apply simp
     apply clarsimp
    apply clarsimp
   apply arith
   prefer 2
   apply clarsimp
  apply (clarsimp simp: nat_distrib)
  apply (frule lem)
  apply arith
  done

end
